\documentclass{article}
\usepackage[margin=.5in]{geometry}
\usepackage{amsmath}
\usepackage{mathtools}
\usepackage{tabularx}

% https://tex.stackexchange.com/questions/89166/centering-in-tabularx-and-x-columns/89168
\newcolumntype{Y}{>{\centering\arraybackslash}X}

\begin{document}


\section{Poisson-normal}

\begin{align*}
\eta_{ij} & = \log{\mu_{ij}} + b_j + e_{ij} \\
b_j & \sim N\left(0, \tau^2\right) \\
e_{ij} & \sim N\left(0, \sigma^2\right) \\
\eta_{ij} & = \log{\lambda_{ij}} \\
\lambda_{ij} & = \exp{\eta_{ij}} \\
\left.y_{ij} \middle| b_j\right. & \sim \text{Poisson}\left(\lambda_{ij}\right)
\end{align*}

\begin{align*}
\text{E}\left(y_{ij} \middle| b_j\right) = \lambda_{ij} \\
\text{Var}\left(y_{ij} \middle| b_j\right) = \lambda_{ij}
\end{align*}

\begin{align*}
\text{E}\left(\lambda\right) & = \exp{\left(\log{\mu}+\left(\tau^2+\sigma^2\right) / 2\right)} \\
\text{Var}\left(\lambda\right) & = \exp{\left(2 \log{\mu} + 2\tau^2 + 2\sigma^2\right)} - \exp{\left(2\log{\mu} + \tau^2 +\sigma^2 \right)}
\end{align*}
%
%\begin{align*}
%\text{E}\left(y\right) & = \text{E}\left(\lambda\right) \\
%& = \exp{\left(\log{\mu}+\left(\tau^2 + \sigma^2\right) / 2\right)} \\
%& = \mu \exp{\left(\tau^2 / 2\right)} \exp{\left(\sigma^2 / 2\right)}
%\end{align*}
%
%\begin{align*}
%\text{Var}\left(y\right) & = \text{Var}\left(\text{E}\left(y_{ij} \middle| b_j\right)\right) +
%  \text{E}\left(\text{Var}\left(y_{ij} \middle| b_j\right)\right) \\
%& = \text{Var}\left(\lambda\right) +
%  \text{E}\left(\lambda\right) \\
%& = \exp{\left(\log{\mu}+\left(\tau^2+\sigma^2\right) / 2\right)} +
%  \exp{\left(2 \log{\mu} + 2\tau^2+2\sigma^2 \right)} -
%  \exp{\left(2\log{\mu} + \tau^2+\sigma^2\right)} \\
%& = \mu \exp\left(\tau^2 / 2\right) \exp\left(\sigma^2 / 2\right) +
%  \mu^2 \left(\exp\left(2\tau^2 + 2\sigma^2\right) - \exp{\left(\tau^2 + \sigma^2\right)} \right) \\
%& = \mu^2 \left(\exp\left(2\tau^2 + 2\sigma^2\right) - \exp{\left(\tau^2 + \sigma^2\right)} \right) +
%  \mu \exp\left(\tau^2 / 2\right) \exp\left(\sigma^2 / 2\right)
%\end{align*}

%%%%%%%%%%%%%%%%%%%%%%%%%%%%%%%%%%

\section{Poisson-gamma}
\begin{align*}
\eta_{ij} & = \log{\mu_{ij}} + b_j \\
b_j & \sim N\left(0, \tau^2\right) \\
u_{ij} & \sim \Gamma\left(\phi, \text{rate}=\phi\right) \\
\eta_{ij} & = \log{\left(\lambda_{ij} u_{ij} \right)} = \log{\lambda_{ij}} + \log{u_{ij}} \\
\lambda_{ij} u_{ij} & = \exp{\eta_{ij}} \\
\left.y_{ij} \middle| b_j, u_{ij}\right. & \sim \text{Poisson}\left(\lambda_{ij} u_{ij}\right) \\
\left.y_{ij} \middle| b_j \right. & \sim \text{Negative Binomial}\left(\lambda_{ij}, \phi\right)
\end{align*}

\begin{align*}
\text{E}\left(y_{ij} \middle| b_j\right) & = \lambda_{ij} \\
\text{Var}\left(y_{ij} \middle| b_j\right) & = \lambda_{ij} + \lambda_{ij}^2 / \phi
\end{align*}


%%%%%%%%%%%%%%%%%%%%%%%%

\begin{align*}
\text{E}\left(\lambda\right) & = \exp{\left(\log{\mu}+\left(\tau^2\right) / 2\right)} \\
\text{Var}\left(\lambda\right) & = \exp{\left(2 \log{\mu} + 2\tau^2 \right)} - \exp{\left(2\log{\mu} + \tau^2 \right)}
\end{align*}

\begin{align*}
\text{E}\left(y\right) & = \exp{\left(\log{\mu}+\left(\tau^2\right) / 2\right)} \\
\text{Var}\left(y\right) & = \text{E}\left(\text{Var}\left(y_{ij} \middle| b_j \right)\right) +
                                 \text{Var}\left(\text{E}\left(y_{ij} \middle| b_j \right)\right) \\
                        & = \text{E}\left(\lambda_{ij} + \lambda_{ij}^2 / \phi\right) +
                            \text{Var}\left(\lambda\right) \\
                        & = \text{E}\left(\lambda\right)+\phi^{-1} \text{E}\left(\lambda^2\right) + \text{Var}\left(\lambda\right) \\
                        & = \text{E}\left(\lambda\right)+\phi^{-1}\text{Var}\left(\lambda\right) + \phi^{-1}\text{E}\left(\lambda\right)^2 + \text{Var}\left(\lambda\right) \\
                        & = \text{E}\left(\lambda\right) + \phi^{-1}\text{E}\left(\lambda\right)^2 + \text{Var}\left(\lambda\right)\left(1 + \phi^{-1}\right)
\end{align*}

\end{document}
